# Ejercicio 11

```
join [] = []
join (xs : xss) = xs ++ join xss

singleton x = [x]

-- Extra

map _ [] = []
map f (x : xs) = f x : map f xs

(++) []     ys = ys
(++) (x:xs) ys = x : xs ++ ys
```

## a. Demostración: id = join . map singleton

### Caso base []

```
(join . map singleton) []
= <def. .>
join (map singleton [])
= <def. map .1>
join []
= <def. join .1>
[]
```

### Paso inductivo xs : xss

#### HI: (join . map singleton) xss = id xss

```
(join . map singleton) (xs : xss)
= <def. .>
join (map singleton (xs : xss))
= <def. map .2>
join ((singleton xs) : (map singleton xss))
= <def. join .1>
singleton xs ++ join (map singleton xss)
= <def. .>
singleton xs ++ (join . map singleton) xss
= <HI>
singleton xs ++ id xss
= <def id., def. singleton>
[xs] ++ xss
= <prop.>
xs : xss
= <def. id>
id (xs : xss)

Propiedad:
[xs] ++ xss
= <syntactic sugar>
(xs : []) ++ xss
= <def. ++ .2>
xs : [] ++ xss
= <def. ++ .1>
xs : xss
```

## b. Demostración: join . join = join . map join

### Caso base []

```
(join . map join) []
= <def. .>
join (map join [])
= <def. map .1>
join []
= <def. join .1>
[]
```

### Paso inductivo xs : xss

#### HI: (join . join) xss = (join . map join) xss

```
(join . map join) (xs : xss)
= <def. .>
join (map join (xs : xss))
= <def. map .2>
join (join xs : map join xss)
= <def. join .2>
join xs ++ join (map join xss)
= <def. .>
join xs ++ (join . map join) xss
= <HI>
join xs ++ (join . join) xss
= <def. .>
join xs ++ join (join xss)
= <def. join .2>
join (xs : join xss)
= <def. ++ .1, syntactic sugar>
join (xs : [] ++ join xss)
= <def. ++ .1>
join (xs ++ join xss)
= <def. join .2>
join (join (xs : xss))
= <def .>
(join . join) (xs : xss)
```